We have the following numbers already from the exercise above:
\begin{align*}
  p(a,b,c) &= 0.096 \\
  p(a) &= 0.4 \\
  p(a,c) &= 0.16 \\
  p(c) &= 0.52 \\
  p(b,c) &= 0.312
\end{align*}
We can calculate the following:
\begin{align*}
  p(c|a) &= \frac{p(a,c)}{p(a)} = \frac{0.16}{0.4} = 0.4 \\
  p(b|c) &= \frac{p(b,c)}{p(c)} = \frac{0.312}{0.52} = 0.6
\end{align*}
Now we simply calculate $p(a)p(c|a)p(b|c)$ and $p(a,b,c)$:
\begin{align*}
  p(a)p(c|a)p(b|c) &= 0.4 \cdot 0.6 \cdot 0.4 = 0.096 \\
  p(a,b,c) &= 0.096 \\
\end{align*}
Thus we have shown that $p(a)p(c|a)p(b|c) = p(a,b,c)$. The graph is shown below.\\
\begin{tikzpicture}

  \begin{scope}[every node/.style={circle,thick,draw}]
    \node (A) at (0,0) {A};
    \node (B) at (3,0) {B};
    \node (C) at (1.5,2) {C};
  \end{scope}

  \begin{scope}[>={Stealth[black]},
              every edge/.style={draw=red,very thick}]
    \path [->] (A) edge node {} (C);
    \path [->] (C) edge node {} (B);
  \end{scope}

\end{tikzpicture}
