To find the pdf of the cdf $F$, we have to look at the definition, where $f$ is the pdf:
$$
F' = f
$$
This means we have to find the derivative of:
$$
F(x) =
\left\{
\begin{array}{ll}
0, & x \leq 0 \\
1 - e^{- (\beta x)^\alpha}, & x > 0
\end{array}
\right.
$$
With respect to $x$:
$$
f(x) =
\left\{
\begin{array}{ll}
\frac{d}{dx} 0, & x \leq 0 \\
\frac{d}{dx} 1 - e^{- (\beta x)^\alpha}, & x > 0
\end{array}
\right.
$$
$$
f(x) =
\left\{
\begin{array}{ll}
0, & x \leq 0 \\
\frac{\alpha e^{-(\beta x)^\alpha} (\beta x)^\alpha}{x}, & x > 0
\end{array}
\right.
$$