To find the median, we have to look at the definition:
$$
median := F(m) = \frac{1}{2}
$$
We can write this out, and try to solve for $m$:
$$
F(m) = 1 - e^{-(\beta m)^{\alpha}} = \frac{1}{2}
$$
$$
1 = \frac{1}{2} + e^{-(\beta m)^{\alpha}}
$$
$$
ln(1) = ln\left(\frac{1}{2}\right) + ln(e^{-(\beta m)^\alpha})
$$
$$
0 - ln\left(\frac{1}{2}\right)= ln(e^{-(\beta m)^\alpha})
$$
$$
ln(2) = -(\beta m)^\alpha
$$
Since $\alpha, \beta > 0$ we can do the following:
$$
\frac{\sqrt[\alpha]{ln(2)}}{\beta} = m
$$