To prove that $\hat{\theta}_{stupid}$ is an unbiased estimator, we first have to look at the definition of such:
$$
BIAS(\hat{\theta}_{stupid}) = \mathbb{E}\hat{\theta}_{stupid} - \theta_0 = 0
$$
We will rewrite this, using the fact that we know the following: 
$$
\theta_0 = \mathbb{E}X_1
$$
$$
\mathbb{E}\hat{\theta}_{stupid} = \mathbb{E}\frac{1}{3} \sum_{i=1}^3
$$
We can now see that we have to prove the following:
$$
\mathbb{E}\left(\frac{1}{3} \sum_{i=1}^3\right) - \mathbb{E}X_1 = 0
$$
Since we know that $(X_1, X_2, X_3)$ are identically distributed, we can say the following:
$$
\mathbb{E}X_1 = \mathbb{E}X_n
$$
Thus, we can finalise the proof:
$$
\frac{\mathbb{E}X_1 + \mathbb{E}X_2 + \mathbb{E}X_3}{3} - \mathbb{E}X_1 = \mathbb{E}X_1 - \mathbb{E}X_1 = 0
$$