To prove this, we need to state a few things:\\
We know that it is possible to convert the basis a vector is shown in, by multiplying the vector onto the new basis $B =\{b_1,b_2\}$. We will do the following:\\\\
First we will show that $(x-y) = (x_b-y_b)$. We do this by making a combined vector of $(x-y)$:
$$
(x-y) = 
\begin{pmatrix}
x_1-y_1\\
x_2-y_2
\end{pmatrix}
$$
Now we can show the vector $(x-y)$ by showing $B(x-y)$:\\
$$
B(x-y) =
\begin{bmatrix}
(b_1)_1 & (b_2)_1\\
(b_1)_2 & (b_2)_2
\end{bmatrix}
\begin{bmatrix}
x_1-y_1\\
x_2-y_2
\end{bmatrix}
=
\begin{bmatrix}
(b_1)_1(x_1-y_1) + (b_2)_1(x_2-y_2)\\
(b_1)_2(x_1-y_1) + (b_2)_2(x_2-y_2)
\end{bmatrix}
= (x_b-y_b)
$$
Since we have shown that $(x-y)=(x_b-y_b)$ we can say the following:
$$
||x-y|| = \sqrt{x^2}-\sqrt{y^2} = \sqrt{x^2_b}-\sqrt{y^2_b} = ||x_b-y_b||
$$