\subsubsection{i)}
To show that $E(f_W)=(Xw-y)^T(Xw-y)$, we will first write this out according to the error function given, part by part. First of all, we will define $D$ as the highest value of $d$, to avoid confusion. Now, $f_w(x)$ can be written in a more useful way:
$$
f_w(x_n) = w_1x_n+w_2x_n^2+...+w_Dx_n^D = \sum_{d=1}^D w_d x_n^d
$$
This can be set into the error function:
$$
E(f_w) = \sum_{n=1}^N (y_n-f(x_n))^2 = \sum_{n=1}^N \Big(y_n-\Big(\sum_{d=1}^D w_d x_n^d\Big)\Big)^2
$$
Now, we will show this backwards, by rewriting $(Xw-y)^T(Xw-y)$ to $E(f_w)$. First we will write the mathematical expression for each element in the resulting vector $Xw$:
$$
Xw_n =
\left[
\begin{array}{llll}
x_1    & x_1^2  & \dots  & x_1^d  \\
x_2    & x_2^2  & \dots  & x_2^d  \\
\vdots & \vdots & \ddots & \vdots \\
x_N    & x_N^2  & \dots  & x_N^d  \\
\end{array}
\right]
\left[
\begin{array}{l}
w_1\\
w_2\\
\vdots\\
w_d
\end{array}
\right]
=
w_1x_n+w_2x_n^2+...+w_Dx_n^D = \sum_{d=1}^D w_d x_n^d
$$
We can see that this is the same as $f_w(x_n)$, and will substitute that following. Since $\sum_{d=1}^D w_d x_n^d$ is only the expression for a single element in $Xw$, we can write the vector as thus:
$$
Xw = 
\left(
\begin{array}{l}
f_w(x_1) \\
f_w(x_2) \\
\vdots \\
f_w(x_n)
\end{array}
\right)
$$
Then, $Xw-y$ must look like this:
$$
(Xw-y)= 
\left(
\begin{array}{l}
f_w(x_1)-y_1 \\
f_w(x_2)-y_2 \\
\vdots \\
f_w(x_n)-y_n
\end{array}
\right)
$$
Now, to write $(Xw-y)^T(Xw-y)$, we can see the following:
$$
\left(
\begin{array}{l}
f_w(x_1)-y_1 \\
f_w(x_2)-y_2 \\
\vdots \\
f_w(x_n)-y_n
\end{array}
\right)^T
\left(
\begin{array}{l}
f_w(x_n)-y_1 \\
f_w(x_n)-y_2 \\
\vdots \\
f_w(x_n)-y_n
\end{array}
\right)
= \sum_{n=1}^N\Big(f_w(x_n)-y_n\Big)^2
$$
We know that $a^2 = (-a)^2$, so we can rewrite it as thus:
$$
\sum_{n=1}^N\Big(-f_w(x_n)+y_n\Big)^2 = \sum_{n=1}^N\Big(y_n-f_w(x_n)\Big)^2
$$
Which is exactly what we wanted to show:
$$
E(f_w) = (Xw-y)^T(Xw-y) = \sum_{n=1}^N\Big(y_n-f_w(x_n)\Big)^2
$$
\subsubsection{ii)}
For this part of the exercise, the proof has not been finished, but here is as far as I got:\\
We will use $d$ and $D$ the same way here as in the previous exercise, and will define $c = D$:
$$
E(f_w) = \sum_{n=1}^N\bigg(y_n-\Big(\sum_{d=1}^Dw_dx_n^d\Big)\bigg)^2
$$
$$
2X^TXw-2x^Ty =
2
\left(
\begin{array}{l}
\sum_{n=1}^N\sum_{d=1}^Dw_dx_n^dx_n^1 \\
\sum_{n=1}^N\sum_{d=1}^Dw_dx_n^dx_n^2 \\
\vdots \\
\sum_{n=1}^N\sum_{d=1}^Dw_dx_n^dx_n^c 
\end{array}
\right)
-2
\left(
\begin{array}{l}
\sum_{n=1}^Nx_n^1y_n \\
\sum_{n=1}^Nx_n^2y_n \\
\vdots \\
\sum_{n=1}^Nx_n^cy_n \\
\end{array}
\right)
$$
$$
2X^TXw-2x^Ty = 2\Big(\sum_{n=1}^N\sum_{d=1}^Dw_dx_n^dx_n^c\Big)-2\Big(\sum_{n=1}^Nx_n^cy_n\Big)
$$

$$
\nabla E(f_w) = \frac{\partial}{\partial w_d} \sum_{n=1}^N\bigg(y_n-\Big(\sum_{d=1}^Dw_dx_n^d\Big)\bigg)^2 = 2\Big(\sum_{n=1}^N\sum_{d=1}^Dw_dx_n^dx_n^c\Big)-2\Big(\sum_{n=1}^Nx_n^cy_n\Big)
$$




