To prove that $\mathbb{E}Z = argmin_\alpha\mathbb{E}((Z-\alpha)^2)$, we will first write out what that means:
$$
\mathbb{E}Z=\sum_zzp(z)
$$
$$
argmin_\alpha\mathbb{E}((Z-\alpha)^2) = \left(\frac{\partial}{\partial\alpha} \mathbb{E}((Z-\alpha)^2)=0\right)
$$
We will start by expanding the second expression:
$$
\frac{\partial}{\partial\alpha}\mathbb{E}(Z^2-2Z\alpha+a^2) = 0
$$
$$
\frac{\partial}{\partial\alpha}\mathbb{E}(Z^2)-\mathbb{E}(2Z\alpha)+\mathbb{E}(a^2) = 0
$$
Now we will write out the expressions in full:
$$
\frac{\partial}{\partial\alpha}\Big(\sum_zz^2p_z(z)\Big)-\frac{\partial}{\partial\alpha}2\alpha\sum_zzp_z(z)+\frac{\partial}{\partial\alpha}\alpha^2 = 0
$$
Now we will derive it with respect to $\alpha$. $\frac{\partial}{\partial\alpha}\Big(\sum_zz^2p_z(z)\Big) = 0$ because $\frac{\partial}{\partial x}c = 0$ 
$$
0-\frac{\partial}{\partial\alpha}2\alpha\sum_zzp_z(z)+\frac{\partial}{\partial\alpha}\alpha^2 = 0
$$
Now we derive the second part of the expression, using the rule $\frac{\partial}{\partial\alpha}c\alpha = c$
$$
\frac{\partial}{\partial\alpha}2\alpha\sum_zzp_z(z) = 2\sum_zzp_z(z)
$$
To derive the the third part, we use the rule that $\frac{\partial}{\partial\alpha}\alpha^n = n\alpha^{n-1}$
$$
\frac{\partial}{\partial\alpha}\alpha^2 = 2\alpha
$$
Now we can add all this into the expression, and end with this:
$$
-2\sum_zzp_z(z)+2\alpha = 0
$$
We can rewrite this to the following:
$$
\sum_zzp_z(z)= \alpha
$$
This is what we wanted to show, now we have:
$$
argmin_\alpha\mathbb{E}((Z-\alpha)^2) = \sum_zzp_z(z) = \mathbb{E}Z
$$