To find the general solution for the recurrence relation, of the form $p(E)x$, we first rewrite it:
\begin{align*}
  x_n &= 2(x_{n-1}+x_{n-2}) \\
  0 &= -x_n + 2(x_{n-1}+x_{n-2}) \\
  p(\lambda) &=  -\lambda^2 + 2\lambda  + 2
\end{align*}
We then use Wolfram Alpha to solve for $p(\lambda) = 0$:
$$
\lambda_1 = 1 - \sqrt{3}
$$
$$
\lambda_2 = 1 + \sqrt{3}
$$
Thus, the general solution is:
$$
x_n = \alpha(1+\sqrt{3})^n + \beta(1-\sqrt{3})^n
$$
We can determine that the difference equation is unstable since all roots do not satisfy the requirement of being $\leq 1$.
