For this proof we can assume the following:
$$
\{a_n\} \text{ with } lim_{n \rightarrow \infty}a_n = a
$$
And we need to prove that the following is true:
$$
\{-a_n\} \text{ with } lim_{n \rightarrow \infty}-a_n = -a
$$
To do this, we need to prove the following:
$$
|-a_n+a| \leq |a_n-a| < \epsilon
$$
From the definition of limits, we know that the following is true for $a$:\\
For every $\epsilon > 0$ there exists an integer $N \in \mathbb{N}$ such that $|a_n-a| < \epsilon$ for all $n > N$.\\
We know, using the rule that $|a|=|-a|$, that the following must be true:
$$
|a_n-a| = |-(a_n-a)| = |-a_n+a| < \epsilon \implies |-(a_n-a)| < \epsilon
$$
Now that we know this is true, our claim must also be true.