First we want to prove this one way; thus, we want to show that:
$$
|(a_n)_i -a_i| \leq ||a_n-a|| < \epsilon
$$
We assume that: $a_n \to a$ is true, and thus, the definition of convergence must also be true for it, hence $|a_n-a| \leq \epsilon$ must be true.
Since we know that the square root of the sum of all squared numbers in the vector is equal to the length of the vector, we can say the following:
$$
\sqrt{\sum_{i=1}^{d}(a_n)_i^2} \leq ||a_n||
$$
\begin{center}
and
\end{center}
$$
\sqrt{\sum_{i=1}^{d}a_i^2} \leq ||a||
$$
Thus, we can show that:
$$
\sqrt{\sum_{i=1}^{d}(a_n)_i^2} -\sqrt{\sum_{i=1}^{d}a_i^2} \leq ||a_n-a|| < \epsilon
$$
With this, we have shown that:
$$
a_n \to a \implies (a_n)_i \to a_i
$$
Now we have to show the opposite:
$$
(a_n)_i \to a_i \implies a_n \to a
$$
This means that
$$
|(a_n)_i \to a_i| < \epsilon
$$
Following the same rules as before, we can see that we have to prove the following:
$$
|a_n - a| \leq |(a_n)_i - a_i| < \epsilon
$$